theories/heap_lang/lifting.v
@@ -292,7 +292,6 @@ Lemma wp_resolve_proph e1 e2 p v w:
   {{{ p ⥱ v }}} ResolveProph e1 e2 {{{ RET (LitV LitUnit); ⌜v = Some w⌝ }}}.
 Proof.
   iIntros (<- <- Φ) "Hp HΦ". iApply wp_lift_atomic_head_step_no_fork; auto.
-  unfold cons_obs. simpl.
   iIntros (σ1 κ κs) "[Hσ HR] !>". iDestruct "HR" as (R [Hfr Hdom]) "HR".
   iDestruct (@proph_map_valid with "HR Hp") as %Hlookup.
   iSplit; first by eauto.
